src/PlutusIR/Semantics/Static/Context.v
@@ -4,5 +4,5 @@ Require Export PlutusCert.Util.Map.
 Require Export PlutusCert.Util.Map.Mupdate.
 
 (** Kind and type contexts*)
-Definition Delta : Type := partial_map Kind.
+Definition Delta : Type := partial_map kind.
 Definition Gamma : Type := partial_map Ty.
